Lampe/Lampe/Tactic/SLNorm.lean
@@ -1,0 +1,49 @@
+import Lampe.SeparationLogic.State
+import Lampe.SeparationLogic.SLP
+
+namespace Lampe.SLP
+
+namespace Internal
+
+theorem rot_singleton_pure {P : Prop} : ([a ↦ b] ⋆ P) = (P ⋆ [a ↦ b]) := by
+  rw [star_comm]
+
+theorem rot_singleton_pure_star {P : Prop} {Q : SLP (State p)} : ([a ↦ b] ⋆ P ⋆ Q) = (P ⋆ [a ↦ b] ⋆ Q) := by
+  rw [SLP.star_comm, SLP.star_assoc]
+  apply SLP.eq_of_iff <;> {apply SLP.star_mono_l; rw [SLP.star_comm]; apply SLP.entails_self}
+
+theorem rot_forall_pure [LawfulHeap α] {P : Prop} {f : β → SLP α} : (SLP.forall' f ⋆ P) = (P ⋆ SLP.forall' f) := by
+  simp [SLP.star_comm]
+
+theorem rot_forall_pure_star [LawfulHeap α] {P : Prop} {f : β → SLP α} {Q : SLP α} :
+    (SLP.forall' f ⋆ P ⋆ Q) = (P ⋆ SLP.forall' f ⋆ Q) := by
+  rw [SLP.star_comm, SLP.star_assoc]
+  apply SLP.eq_of_iff <;> {apply SLP.star_mono_l; rw [SLP.star_comm]; apply SLP.entails_self}
+
+theorem rot_exists_pure [LawfulHeap α] {P : Prop} {f : β → SLP α} : (SLP.exists' f ⋆ P) = (P ⋆ SLP.exists' f) := by
+  simp [SLP.star_comm]
+
+theorem rot_exists_pure_star {P : Prop} {Q : SLP (State p)} : (SLP.exists' f ⋆ P ⋆ Q) = (P ⋆ SLP.exists' f ⋆ Q) := by
+  rw [SLP.star_comm, SLP.star_assoc]
+  apply SLP.eq_of_iff <;> {apply SLP.star_mono_l; rw [SLP.star_comm]; apply SLP.entails_self}
+
+end Internal
+
+macro "sl_norm" : tactic => `(tactic|(
+  try simp only [
+    star_assoc,
+    star_true,
+    true_star,
+    exists_pure,
+    exists_star,
+    star_exists,
+    Internal.rot_singleton_pure,
+    Internal.rot_singleton_pure_star,
+    Internal.rot_forall_pure,
+    Internal.rot_forall_pure_star,
+    Internal.rot_exists_pure,
+    Internal.rot_exists_pure_star,
+  ]
+))
+
+end Lampe.SLP
